logrel: new interp_access WIP

theories/logrel/logrel.v
@@ -22,14 +22,14 @@ Section logrel.
   destruct hypconst. simpl. lia.
   Defined.
 
-  Definition unknown_mem_page (p: PID):=
-   ([∗ list] a ∈ addr_of_page p, ∃ w, (a ->a w))%I.
-
+  Definition unknown_mem_page (p: PID) :=
+    (∃ mem,
+   [∗ map] a ↦ w ∈ mem,  ⌜a ∈ addr_of_page p⌝ -∗ (a ->a w))%I.
 
   (** definition **)
   Program Definition interp_execute: E :=
-   λne (i: leibnizO VMID), (⌜ fin_to_nat i ≠ 0 ⌝ -∗ (VMProp_holds i (1/2)%Qp -∗ WP ExecI @ i {{(λ _, True )}}))%I.
-
+   λne (i: leibnizO VMID), (⌜ fin_to_nat i ≠ 0 ⌝ -∗
+        (VMProp_holds i (1/2)%Qp -∗ WP ExecI @ i {{(λ _, True )}}))%I.
 
   Definition shared_or_noaccess_pages (i:VMID) (pgt: page_table) : iProp Σ:=
     (
@@ -50,38 +50,60 @@ Section logrel.
                                 p -@EA> i ∗ unknown_mem_page p
     )%I.
 
-  Definition full_reg_map (reg: reg_file) : iProp Σ := (∀ (r: reg_name), ⌜is_Some (reg !! r)⌝)%I.
 
-  Definition full_pgt_map (pgt: page_table) : iProp Σ := (∀ (p: PID), ⌜is_Some (pgt !! p)⌝)%I.
+  (* FIXME: replace gmap *)
+
+  Definition total_reg_map (reg: gmap reg_name Addr) : iProp Σ := (∀ (r: reg_name), ⌜is_Some (reg !! r)⌝)%I.
+
+  Definition total_pgt_map (pgt: gmap PID (VMID * (gset VMID))) : iProp Σ := (∀ (p: PID), ⌜is_Some (pgt !! p)⌝)%I.
+
+  Definition total_mem_map (mem: gmap Addr Word) : iProp Σ := (∀ (a: Addr), ⌜is_Some (mem !! a)⌝)%I.
 
   Program Definition interp_access: V :=
     λne (i:leibnizO VMID) (pgt: page_table),
-    ( (* registers *)
-        (∃ regs, full_reg_map regs ∗ [∗ map] r ↦ w ∈ regs, r @@i ->r w) ∗
-         full_pgt_map pgt ∗
-        (* VMProp  *)
-        VMProp i (
-          (* in case of yielding, we need the following to apply yield rule*)
-          (* R0 & R1 of pvm *)
-          (R0 @@ V0 ->r encode_hvc_func(Run) ∗ R1 @@ V0 ->r encode_vmid(i) ∗
-          (* VMProp of pvm *)
-          (* if i yielding, we give following resources back to pvm *)
-          VMProp V0 (
-            (* R0 and R1 of pvm *)
-            R0 @@ V0 ->r encode_hvc_func(Yield) ∗ R1 @@ V0 ->r encode_vmid(i) ∗
-            (* exclusive access pagetable entries + mem *)
-            (exclusive_access_pages i pgt) ∗
-            (* shared/noaccess pagetable entries + shared mem *)
-            (shared_or_noaccess_pages i pgt)
-              (* TODO: recursive definition *)
-          ) (1/2)%Qp ∗
-          (* exclusive access pagetable entries + mem *)
-          (exclusive_access_pages i pgt) ∗
-          (* shared/noaccess pagetable entries + shared mem *)
-          (shared_or_noaccess_pages i pgt))
-          (* no scheduling, we finish the proof *)
-          ∨ False
-        ) (1/2)%Qp
-      )%I.
+    (∃ regs pgt_act shandle,
+      (* registers *)
+      (total_reg_map regs ∗ [∗ map] r ↦ w ∈ regs, r @@ i ->r w) ∗
+      (* mailbox *)
+      (∃ p, RX@i := p) ∗ (∃ p, TX@i := p) ∗
+      (* pgt, considering mem sharing *)
+      ⌜dom (gset PID) pgt = dom (gset PID) pgt_act⌝ ∗
+      (* pgt is the upper bound of pgt_act in terms of accessibility of VM i*)
+      ([∗ map] p ↦ pe ∈ pgt, ⌜i ∉ pe.2⌝ -∗ ⌜pgt_act !! p = Some pe⌝) ∗
+      ([∗ map] p ↦ pe ∈ pgt, ⌜i ∈ pe.2⌝ -∗
+        (∃ (pe_act: (VMID * gset VMID)), ⌜pgt_act !! p = Some pe_act⌝ ∗ ⌜pe.1 = pe_act.1⌝ ∗ (⌜pe_act.2 = pe.2⌝
+           ∨ (⌜pe_act.2 = pe.2 ∖ {[i]}⌝ ∗ (∃wh v x y m f, wh->t{1}( v , x , y , m , f ) ∗ ⌜wh ∉ shandle⌝ ∨ True))))) ∗
+      (* handle pool *)
+      hp{1}[shandle] ∗
+      (* VMProp *)
+      VMProp i (
+        (* pagetable is total *)
+        total_pgt_map pgt ∗
+        (* memory is total *)
+        (* total_mem_map mem ∗ *)
+        (* in case of yielding, we need the following to apply yield rule*)
+        (* R0 & R1 of pvm *)
+        (R0 @@ V0 ->r encode_hvc_func(Run) ∗ R1 @@ V0 ->r encode_vmid(i) ∗
+        (* VMProp of pvm *)
+        (* if i yielding, we give following resources back to pvm *)
+        VMProp V0 (
+          (* R0 and R1 of pvm *)
+          R0 @@ V0 ->r encode_hvc_func(Yield) ∗ R1 @@ V0 ->r encode_vmid(i) ∗
+           (* exclusive access pagetable entries + mem *)
+           (exclusive_access_pages i pgt_act) ∗
+           (* shared/noaccess pagetable entries + shared mem *)
+           (shared_or_noaccess_pages i pgt_act)
+               (* NOTE: if i will be scheduled arbitrary number of times, need recursive definition *)
+               ) (1/2)%Qp ∗
+        (* exclusive access pagetable entries + mem *)
+        (exclusive_access_pages i pgt_act) ∗
+        (* shared/noaccess pagetable entries + shared mem *)
+        (shared_or_noaccess_pages i pgt_act) ∗
+        (* status of RX *)
+        (RX@ i :=() ∨ ∃ w s, RX@ i :=(w, s)))
+        (* no scheduling, we finish the proof *)
+        ∨ False
+      ) (1/2)%Qp
+    )%I.
 
 End logrel.
