theories/logrel/fundamental.v
@@ -13,133 +13,78 @@ Section fundamental.
   Context `{vmG: !gen_VMG Σ}.
 
   (* TODO: separate into helper lemmas *)
-  Lemma ftlr (i:VMID) (pgt:page_table) :
-    interp_access i pgt ⊢ interp_execute i.
+  Lemma ftlr (i:VMID)  :
+   ∀ pgt, interp_access i pgt ⊢ interp_execute i.
   Proof.
     rewrite /interp_access /=.
-    iLöb as "IH". 
-    iIntros "((%reg & #Hfull_regs & regs) & %Hfull_pgt & VMProp) Hnotp VMProp_holds".
-    iDestruct (VMProp_holds_agree i with "[VMProp_holds VMProp]") as "[Hres VMProp]".
-    { iFrame. }
-    iDestruct( later_or with "Hres") as "Hres".
+    iLöb as "IH".
+    iIntros (pgt) "(%regs & (#Htotal_regs & regs) & rx & tx & VMProp) Hnotp VMProp_holds".
+    iDestruct (VMProp_holds_agree i with "[$VMProp_holds $VMProp]") as "[Hres VMProp]".
+    iDestruct( later_exist with "Hres") as (mem) "Hres".
+    iDestruct (later_or with "Hres") as "Hres".
     iDestruct "Hres" as "[Hres| >False]";last done.
     (* the vm is scheduled *)
     rewrite !later_sep.
     (* we have to do this because VMProp is not(?) timeless *)
-    iDestruct "Hres" as "(>R0z & >R1z & (VMPropz & >excl_pages & >shared_pages))".
+    iDestruct "Hres" as "(>#Htotal_pgt & >#Htotal_mem & >R0z & >R1z & (VMPropz & >excl_pages & >shared_pages & >rx_status))".
     (* we don't really need to get the resource of PC, but just the value *)
-    iPoseProof ("Hfull_regs" $! PC) as "%Hlookup_PC".
+    iPoseProof ("Htotal_regs" $! PC) as "%Hlookup_PC".
     destruct Hlookup_PC as [ai Hlookup_PC].
     (* getting sacc from pgt *)
-    pose proof (Hfull_pgt (to_pid_aligned ai)) as Hlookup_ai.
-    simpl in Hlookup_ai.
+    iPoseProof ("Htotal_pgt" $! (to_pid_aligned ai)) as "%Hlookup_ai".
     destruct Hlookup_ai as [[? sacc] Hlookup_ai].
     (* sswp *)
-    rewrite wp_sswp.
+    rewrite ->wp_sswp.
     destruct (decide (i ∈ sacc)).
     { (* i has access *)
-      destruct (decide (sacc = {[i]})) as [Heqs | Heqs].
+      destruct (decide (sacc = {[i]})) as [->Heqs | Heqs].
       { (* i has exclusive access *)
-        iEval(rewrite /exclusive_access_pages) in "excl_pages".        
-        rewrite (big_opM_delete _ _ (to_pid_aligned ai) _ Hlookup_ai).
-        iDestruct ("excl_pages") as "[pi excl_pages]".
-        simpl.
-        iDestruct ("pi" with "[]") as "[pi pi_mem]";first done.
-        rewrite /unknown_mem_page.
-        pose proof (in_page_to_pid_aligned ai) as Hinpage_ai.
-        pose proof (addr_of_page_NoDup (tpa ai)) as HNoDup_ai.
-        rewrite -big_opS_list_to_set; last exact HNoDup_ai.
-        rewrite big_opS_delete.
-        Unshelve.
-        3 : { exact ai. }
-        2 : {
-          apply elem_of_list_to_set.
-          apply tpa_addr_of_page.
-          (* apply of_pid_tpa_addr_of_page. *)
-        }
-        iDestruct "pi_mem" as "((%instr & instrp) & pi_mem)".
+        iEval(rewrite /exclusive_access_pages) in "excl_pages".
+        iPoseProof ("Htotal_mem" $! ai) as "[%instr %Hlookup_instr]".
         destruct (decode_instruction instr) as [instr'|] eqn:Heqn.
         { (* valid instruction *)
           destruct instr'.
           { (* NOP *)
             (* getting the PC *)
-            iDestruct (reg_bigM_split reg i PC ai Hlookup_PC with "[$Hfull_regs $regs]") as "[PC Hregs_restore]".
-            iApply (nop ai (w1 := instr) (s := sacc) (q := 1%Qp) with "[PC pi instrp]"); auto.
-            rewrite Heqs.
+            iDestruct (reg_big_sepM_split regs i Hlookup_PC with "[$Htotal_regs $regs]")
+              as "[PC Hregs_restore]".
+            (* getting pgt *)
+            iDestruct (pgt_big_sepM_split pgt Hlookup_ai with "[$Htotal_pgt $excl_pages]")
+                       as "[pi Hacc_pgt]".
+            (* getting mem *)
+            iDestruct ("pi" with "[]") as "[pi pi_mem]";first done.
+            rewrite /unknown_mem_page.
+            iDestruct (mem_big_sepM_split mem Hlookup_instr with "[$Htotal_mem $pi_mem]")
+                      as "[instrm Hacc_mem]".
+            iDestruct ("instrm" with "[]") as "instrm".
+            { iPureIntro. apply tpa_addr_of_page. }
+            iApply (nop ai (w1 := instr) (s := {[i]}) (q := 1%Qp) with "[PC pi instrm]"); auto.
             iFrame.
             iSimpl.            
             iNext.
-            iIntros "(PC & instrp & pi) _".
+            iIntros "(PC & instrm & pi) _".
             iDestruct ("Hregs_restore" $! (ai ^+ 1)%f with "PC") as (regs') "regs".
-            iAssert (full_pgt_map pgt ∗ exclusive_access_pages i pgt)%I with "[pi_mem instrp excl_pages pi]" as "[Hpt Hexcl]".
-            {              
-              pose proof (big_opS_insert (fun x => (∃ w, x ->a w)%I) (list_to_set (addr_of_page (tpa ai)) ∖ {[ai]}) ai) as Hrewrite.
-              cbv beta in Hrewrite.
-              iAssert (∃ w : Addr, ai ->a w)%I with "[instrp]" as "instrp".
-              {
-                by iExists instr.                
-              }
-              iCombine "instrp pi_mem" as "instrp".
-              rewrite <-Hrewrite.
-              - unfold full_pgt_map.
-                iSplit.
-                iIntros (p).
-                iPureIntro.
-                specialize (Hfull_pgt p).
-                by simpl in Hfull_pgt.
-                unfold exclusive_access_pages.
-                unfold unknown_mem_page.
-                pose proof (big_opM_fn_insert (o := bi_sep) (fun k y _ => (⌜{[i]} = y.2⌝ -∗ k -@EA> i ∗ ([∗ list] a ∈ addr_of_page k, ∃ w : Addr, a ->a w))%I) (fun _ => True) (delete (tpa ai) pgt) (tpa ai) (v, sacc)) as Hrewrite'.
-                specialize (Hrewrite' True).
-                feed specialize Hrewrite'.
-                unfold page_table in *.
-                apply lookup_delete.
-                cbn in Hrewrite'.
-                set s := list_to_set (addr_of_page (tpa ai)) : gset Addr.
-                assert (({[ai]} ∪ s ∖ {[ai]}) = s) as ->.
-                {
-                  symmetry.
-                  apply union_difference_singleton_L.
-                  subst s.
-                  apply elem_of_list_to_set.
-                  apply tpa_addr_of_page.
-                }
-                subst s.
-                iAssert (⌜{[i]} = sacc⌝ -∗ tpa ai -@EA> i ∗ ([∗ list] a ∈ addr_of_page (tpa ai), ∃ w : Addr, a ->a w))%I with "[pi instrp]" as "H2".
-                {
-                  iIntros.
-                  rewrite Heqs.
-                  iFrame.
-                  rewrite <-big_opS_list_to_set; last exact HNoDup_ai.
-                  iFrame.
-                }
-                iCombine "H2 excl_pages" as "excl_pages".
-                rewrite <-Hrewrite'.
-                rewrite insert_delete_insert.
-                assert (<[tpa ai := (v, sacc)]> pgt = pgt) as H1.
-                {
-                  rewrite insert_id; auto.
-                }
-                rewrite H1.
-                iFrame.
-              - intros c.
-                rewrite ->elem_of_difference in c.
-                destruct c as [_ c].
-                apply c.
-                by apply elem_of_singleton_2.
-            }
+            iDestruct ("Hacc_mem" $! instr with "[instrm]") as (mem') "[#Htotal_mem' pi_mem]".
+            {  iIntros "Hin". iFrame "instrm". }
+            iDestruct ("Hacc_pgt" $! (v,{[i]}) with "[pi pi_mem]") as (pgt') "[pgt mem]".
+            (* NOTE: accessor doesn't work on pagetable, since we could update mem.
+               We could solve it by moving the existential into sepM. But it means losing the capability to destruct on instr before split
+             pagetable sepM, which further implies one more splitting is needed. So we cannot use accessor anymore. *)
+            (* But why do we use accessor here? IH doesn't need pgt and mem as they are in VMProp!! *)
+            { iIntros "?". iFrame "pi". (* here accessor needs mem, we have mem' instead. *) admit. }
             iDestruct (VMProp_split with "VMProp") as "[VMProp1 VMProp2]".
-            iSpecialize ("IH" with "[regs Hpt VMProp1]").
-            iFrame.
+            iSpecialize ("IH" $! pgt' with "[regs $rx $tx VMProp1]").
             iExists regs'.
-            iFrame.
+            admit.
+            (* iFrame "VMProp1". *)
             iSpecialize ("IH" with "Hnotp").
-            iEval (rewrite <-wp_sswp) in "IH".
+            (* iEval (rewrite <-wp_sswp) in "IH". *)
             iApply "IH".
             set Pred := (X in VMProp i X _).
             iExists Pred.
             iFrame.
             iNext.
+            iExists mem'.
             iLeft.
             iFrame.
           }
@@ -162,10 +107,10 @@ Section fundamental.
                 naive_solver.
               }
               {
-                iPoseProof ("Hfull_regs" $! (R n fin)) as (w) "%Hlookup_R".
+                iPoseProof ("Htotal_regs" $! (R n fin)) as (w) "%Hlookup_R".
                 (* getting the R *)
-                iDestruct ((reg_bigM_split2 reg i PC ai (R n fin) w _ Hlookup_PC Hlookup_R) with "[$Hfull_regs $regs]")
-                  as "(PC & R & Hregs_restore)".
+                iDestruct ((reg_bigM_split2 reg i PC ai (R n fin) w _ Hlookup_PC Hlookup_R)
+                            with "[$Htotal_regs $regs]") as "(PC & R & Hregs_restore)".
                 iApply (mov_word (w3 := w) _ imm (R n fin) with "[PC pi instrp R]"); iFrameAutoSolve.
                 set_solver.
                 iSimpl.            
@@ -175,7 +120,8 @@ Section fundamental.
                 {
                   iFrame.
                 }
-                iAssert (full_pgt_map pgt ∗ exclusive_access_pages i pgt)%I with "[pi_mem instrp excl_pages pi]" as "[Hpt Hexcl]".
+                iAssert (total_pgt_map pgt ∗ exclusive_access_pages i pgt)%I
+                  with "[pi_mem instrp excl_pages pi]" as "[Hpt Hexcl]".
                 {              
                   pose proof (big_opS_insert (fun x => (∃ w, x ->a w)%I) (list_to_set (addr_of_page (tpa ai)) ∖ {[ai]}) ai) as Hrewrite.
                   cbv beta in Hrewrite.
@@ -185,12 +131,12 @@ Section fundamental.
                   }
                   iCombine "instrp pi_mem" as "instrp".
                   rewrite <-Hrewrite.
-                  - unfold full_pgt_map.
+                  - unfold total_pgt_map.
                     iSplit.
                     iIntros (p).
                     iPureIntro.
-                    specialize (Hfull_pgt p).
-                    by simpl in Hfull_pgt.
+                    specialize (Htotal_pgt p).
+                    by simpl in Htotal_pgt.
                     unfold exclusive_access_pages.
                     unfold unknown_mem_page.
                     pose proof (big_opM_fn_insert (o := bi_sep) (fun k y _ => (⌜{[i]} = y.2⌝ -∗ k -@EA> i ∗ ([∗ list] a ∈ addr_of_page k, ∃ w : Addr, a ->a w))%I) (fun _ => True) (delete (tpa ai) pgt) (tpa ai) (v, sacc)) as Hrewrite'.
@@ -252,7 +198,7 @@ Section fundamental.
           all: admit.
         }
         { (*invalid instruction *)
-          iDestruct (reg_bigM_split reg i PC ai Hlookup_PC with "[$Hfull_regs $regs]") as "[PC _]".
+          iDestruct (reg_bigM_split reg i PC ai Hlookup_PC with "[$Htotal_regs $regs]") as "[PC _]".
           iApply (not_valid_instr (s := sacc) (q := 1%Qp) _ ai instr with "[PC pi instrp]"); auto.
           {
             rewrite Heqs.
@@ -274,7 +220,7 @@ Section fundamental.
       iDestruct ("shared_pages") as "[[pi _] shared_pages]".
       simpl.
       iDestruct ("pi" with "[]") as "pi"; first done.
-      iDestruct (reg_bigM_split reg i PC ai Hlookup_PC with "[$Hfull_regs $regs]") as "[PC _]".
+      iDestruct (reg_bigM_split reg i PC ai Hlookup_PC with "[$Htotal_regs $regs]") as "[PC _]".
       iApply (not_valid_pc with "[PC pi]");
       [exact n|iFrame|].
       iNext;simpl.
