theories/logrel/logrel_extra.v
@@ -385,14 +385,17 @@ Section logrel_extra.
   Context `{hypparams:!HypervisorParameters}.
   Context `{vmG: !gen_VMG Σ}.
 
-  Lemma reg_bigM_split reg i r w:
-    reg !! r = Some w ->
-    ((full_reg_map reg ∗ [∗ map] k↦y ∈ reg, k @@ i ->r y)%I
-     ⊢  (r @@ i ->r w) ∗ (∀ w', r @@ i ->r w' -∗ ∃ reg', (full_reg_map reg' ∗ [∗ map] k↦y ∈ reg', k @@ i ->r y)))%I.
+  (* we provide lookup, so r and w can be implicit *)
+  Lemma ra_big_sepM_split `{Countable K} { V :Type} (map : gmap K V) (k : K) (v:V)
+        (total:= (λ m, (∀ k,  ⌜is_Some (m !! k)⌝)%I) : gmap K V -> iProp Σ) (f: K -> V -> iProp Σ)
+    :
+    map !! k = Some v ->
+    ((total map ∗ [∗ map] k↦y ∈ map, f k y)%I
+     ⊢  (f k v) ∗ (∀ v', (f k v') -∗ ∃ map', (total map' ∗ [∗ map] k↦y ∈ map', f k y)))%I.
   Proof.
-    iIntros (Hsubseteq) "[%Hfull Hregs]".
-    pose proof (Hfull r) as Hlookup_r.
-    iDestruct (big_sepM_union_acc  reg {[r := w]} (λ k v, k @@ i ->r v)%I with "Hregs") as "[Hsingle Hrestore]".
+    iIntros (Hlookup) "[#Htotal Hregs]".
+    iPoseProof  ("Htotal" $! k) as "Hlookup".
+    iDestruct (big_sepM_union_acc map {[k := v]} f with "Hregs") as "[Hsingle Hrestore]".
     {
       apply insert_subseteq_l ;first done.
       apply map_empty_subseteq.
@@ -402,21 +405,19 @@ Section logrel_extra.
       rewrite big_opM_singleton.
       iFrame.
     }
-    iIntros (w') "Hsingle_upd".
-    iExists ({[r := w']} ∪ reg).
+    iIntros (v') "Hsingle_upd".
+    iExists ({[k := v']} ∪ map).
     iSplitL "".
     {
-       unfold full_reg_map.
-       iPureIntro.
-       intro r0.
-       specialize (Hfull r0).
-       destruct Hfull as [? Hlookup_r0].
-       destruct (decide (r = r0)).
-       - subst r.
+       unfold total_reg_map.
+       iIntros (k0).
+       iDestruct ("Htotal" $! k0) as (?)"Hlookup_k0".
+       destruct (decide (k = k0)).
+       - subst k0.
          simplify_map_eq /=.
          done.
        - simplify_map_eq /=.
-         exists x.
+         iExists x.
          rewrite lookup_union_r.
          done.
          apply lookup_singleton_None.
@@ -431,13 +432,25 @@ Section logrel_extra.
   Qed.
 
 
-  Lemma reg_bigM_split2 reg i r1 w1 r2 w2:
+  (* we provide lookup, so r and w can be implicit *)
+  Lemma reg_big_sepM_split reg i {r w}:
+    reg !! r = Some w ->
+    ((total_reg_map (reg: gmap reg_name Addr) ∗ [∗ map] k↦y ∈ reg, k @@ i ->r y)%I
+     ⊢  (r @@ i ->r w) ∗ (∀ w', r @@ i ->r w' -∗ ∃ reg', (total_reg_map reg' ∗ [∗ map] k↦y ∈ reg', k @@ i ->r y)))%I.
+  Proof.
+    rewrite /reg_file /total_reg_map.
+    iIntros (Hlookup).
+    iApply (ra_big_sepM_split reg r w (λ k v, k @@ i ->r v)%I Hlookup).
+  Qed.
+
+
+  Lemma reg_big_sepM_split2 reg i {r1 w1 r2 w2}:
     r1 ≠ r2 ->
     reg !! r1 = Some w1 ->
     reg !! r2 = Some w2 ->
-    ((full_reg_map reg ∗ [∗ map] k↦y ∈ reg, k @@ i ->r y)%I
+    ((total_reg_map reg ∗ [∗ map] k↦y ∈ reg, k @@ i ->r y)%I
      ⊢  (r1 @@ i ->r w1) ∗ (r2 @@ i ->r w2) ∗
-          (∀ w1' w2', r1 @@ i ->r w1' ∗ r2 @@ i ->r w2'-∗ ∃ reg', (full_reg_map reg' ∗ [∗ map] k↦y ∈ reg', k @@ i ->r y)))%I.
+          (∀ w1' w2', r1 @@ i ->r w1' ∗ r2 @@ i ->r w2'-∗ ∃ reg', (total_reg_map reg' ∗ [∗ map] k↦y ∈ reg', k @@ i ->r y)))%I.
   Proof.
     iIntros (Hneq Hlookup1 Hlookup2) "[%Hfull Hregs]".
     pose proof (Hfull r1) as Hlookup_r1.
@@ -464,7 +477,7 @@ Section logrel_extra.
     iExists ({[r1 := w1'; r2:= w2']} ∪ reg).
     iSplitL "".
     {
-      unfold full_reg_map.
+      unfold total_reg_map.
       iPureIntro.
       intro r0.
       specialize (Hfull r0).
@@ -504,6 +517,107 @@ Section logrel_extra.
       split;done.
     }
   Qed.
+
+ Lemma pgt_big_sepM_split (pgt: gmap PID (VMID * gset VMID)) {p pe} {f: _ -> _ -> iProp Σ}:
+    pgt !! p = Some pe->
+    ((total_pgt_map pgt ∗ [∗ map] k↦y ∈ pgt, f k y)%I
+     ⊢  (f p pe) ∗ (∀ (pe' : VMID * gset VMID) , f p pe' -∗
+                          ∃ (pgt': gmap PID (VMID * gset VMID) ), (total_pgt_map pgt' ∗ [∗ map] k↦y ∈ pgt', f k y)))%I.
+  Proof.
+    rewrite /total_pgt_map.
+    iIntros (Hlookup).
+    iApply (ra_big_sepM_split pgt p pe f Hlookup).
+  Qed.
+
+  (* TODO: the proofs of xxx_big_sepM_splitn are almost identical,
+    make a more general lemma to cover reg, pgt and mem *)
+  (* f is also implicit because coq can infer it from big_sepM *)
+  Lemma pgt_big_sepM_split2 (pgt: gmap PID (VMID * gset VMID)) {p1 p2 pe1 pe2} {f: _ -> _ -> iProp Σ}:
+    p1 ≠ p2 ->
+    pgt !! p1 = Some pe1->
+    pgt !! p2 = Some pe2->
+    ((total_pgt_map pgt ∗ [∗ map] k↦y ∈ pgt, f k y)%I
+     ⊢  (f p1 pe1) ∗ (f p2 pe2)∗ (∀ (pe1' pe2' : VMID * gset VMID) , (f p1 pe1' ∗ f p2 pe2') -∗
+                          ∃ (pgt': gmap PID (VMID * gset VMID) ), (total_pgt_map pgt' ∗ [∗ map] k↦y ∈ pgt', f k y)))%I.
+  Proof.
+    iIntros (Hneq Hlookup1 Hlookup2) "[%Htotal pgt]".
+    pose proof (Htotal p1) as Hlookup_p1.
+    pose proof (Htotal p2) as Hlookup_p2.
+    simplify_map_eq.
+    iDestruct (big_sepM_union_acc pgt {[p1 := pe1 ; p2 := pe2 ]} f with "pgt")
+      as "[Hsingle Hrestore]".
+    {
+      apply insert_subseteq_l ;first done.
+      apply insert_subseteq_l ;first done.
+      apply map_empty_subseteq.
+    }
+    rewrite !big_opM_insert.
+    2: {
+      done.
+    }
+    2: {
+      apply lookup_singleton_None.
+      done.
+    }
+    iDestruct "Hsingle" as "(Hsingle1 & Hsingle2 & _)".
+    iFrame "Hsingle1 Hsingle2".
+    iIntros (pe1' pe2') "Hsingle_upd".
+    iExists ({[p1 := pe1'; p2:= pe2']} ∪ pgt).
+    iSplitL "".
+    {
+      unfold total_pgt_map.
+      iPureIntro.
+      intro p0.
+      specialize (Htotal p0).
+      destruct Htotal as [? Hlookup_p0].
+      destruct (decide (p1 = p0)).
+      - subst p1.
+        simplify_map_eq /=.
+        done.
+      - simplify_map_eq /=.
+        destruct (decide (p2 = p0)).
+        + exists pe2'.
+          rewrite lookup_union_Some_raw.
+          left.
+          subst p0.
+          apply lookup_insert_Some.
+          right.
+          split;first done.
+          apply lookup_insert_Some.
+          left.
+          rewrite Hlookup2 in Hlookup_p0.
+          inversion Hlookup_p0;subst x. done.
+        + exists x.
+          rewrite lookup_union_Some_raw.
+          right.
+          split;last done.
+          rewrite !lookup_insert_None;repeat split;done.
+    }
+    {
+      iApply "Hrestore".
+      iPureIntro. set_solver +.
+      rewrite !big_opM_insert.
+      iDestruct "Hsingle_upd" as "[Hsingle_upd1 Hsingle_upd2]".
+      iFrame.
+      done.
+      done.
+      apply lookup_insert_None.
+      split;done.
+    }
+  Qed.
+
+
+ Lemma mem_big_sepM_split (mem: gmap Addr Word) {a w} {f: _ -> _ -> iProp Σ}:
+    mem !! a = Some w->
+    ((total_mem_map mem ∗ [∗ map] k↦y ∈ mem, f k y)%I
+     ⊢  (f a w) ∗ (∀ (w' : Word) , f a w' -∗
+                          ∃ (mem': gmap Addr Word), (total_mem_map mem' ∗ [∗ map] k↦y ∈ mem', f k y)))%I.
+  Proof.
+    rewrite /total_mem_map.
+    iIntros (Hlookup).
+    iApply (ra_big_sepM_split mem a w f Hlookup).
+  Qed.
+
 
   (*
 TODO: For memory chunks
